ZFinaccessible.v
@@ -75,7 +75,6 @@ apply isOrd_intro; intros.
  exists (x ⊔ y). 
   apply subset_intro.
    apply G_osup2; auto.
-   apply H1.
    
    apply isOrd_osup2; trivial.
 
